proof/equivHybrid.ec
@@ -13,10 +13,11 @@ require import GarbleTools.
 require AdvGate.
 
 lemma hybridEq :
-      forall (Adv <: Gate.Adv),
+      forall (Adv <: Gate.Adv{Dkc.Dkc, AdvGate.Adv}),
         equiv [
           Dkc.Game(Dkc.Dkc, AdvGate.Adv(Adv)).work ~
             Dkc.Game(Dkc.Dkc, AdvGate.Adv(Adv)).work :
+          (glob Adv){1} = (glob Adv){2} /\
           (!Dkc.Dkc.b{1}) /\ (AdvGate.Adv.l{1}=0) /\
           (Dkc.Dkc.b{2}) /\ (AdvGate.Adv.l{2}=1)
           ==> !res{1} = res{2}
@@ -27,7 +28,6 @@ proof.
   inline {1} Dkc.Dkc.preInit.
   inline {1} Dkc.Dkc.get_challenge.
   inline {1} Dkc.Dkc.initialize.
-  inline {1} Dkc.Dkc.encrypt.
   inline {1} AdvGate.Adv(Adv).gen_queries.
   inline {1} AdvGate.Adv(Adv).get_challenge.
   inline {1} AdvGate.Adv(Adv).compute0.
@@ -35,7 +35,6 @@ proof.
   inline {2} Dkc.Dkc.preInit.
   inline {2} Dkc.Dkc.get_challenge.
   inline {2} Dkc.Dkc.initialize.
-  inline {2} Dkc.Dkc.encrypt.
   inline {2} AdvGate.Adv(Adv).gen_queries.
   inline {2} AdvGate.Adv(Adv).get_challenge.
   inline {2} AdvGate.Adv(Adv).compute1.
@@ -44,6 +43,7 @@ proof.
   swap [7..9] -6.
 
   app 3 3 : (
+    (glob Adv){1} = (glob Adv){2} /\
     AdvGate.Adv.c{1} = AdvGate.Adv.c{2} /\
     AdvGate.Adv.fc{1} = AdvGate.Adv.fc{2} /\
     AdvGate.Adv.xc{1} = AdvGate.Adv.xc{2} /\
@@ -52,42 +52,98 @@ proof.
     Dkc.Dkc.b{1} = false /\
     AdvGate.Adv.l{2}=1 /\
     Dkc.Dkc.b{2} = true
-  );[wp;call true (res{1}=res{2});[admit|rnd;skip;trivial]|]. (* Call adv gen_queries *)
+  );
+[wp;call ((glob Adv){1} = (glob Adv){2}) ((glob Adv){1} = (glob Adv){2}/\res{1}=res{2});
+[fun true|rnd;skip];trivial|]. (* Call adv gen_queries *)
 
-  case (Gate.eval (fst (fst query{2})) (snd (fst query{2})) = Gate.eval (fst (snd query{2})) (snd (snd query{2}))). (*good*)
+  case (Gate.queryValid query{1}). (*good*)
 
   rcondt {1} 9;[intros &m;wp;rnd;wp;rnd;skip;trivial|]. (*good*)
   rcondf {1} 11;[admit|]. (* l condition *)
   rcondt {1} 10;[admit|]. (* l condition *)
   rcondt {1} 17;[admit|]. (* While *)
-  rcondt {1} 24;[admit|]. (* While *)
-  rcondf {1} 31;[admit|]. (* While *)
-  rcondt {1} 33;[admit|]. (* good *)
-  rcondf {1} 34;[admit|]. (* l *)
-  rcondt {1} 33;[admit|]. (* l *)
+  rcondt {1} 20;[admit|]. (* While *)
+  rcondf {1} 23;[admit|]. (* While *)
+  rcondt {1} 25;[admit|]. (* good *)
+  rcondf {1} 26;[admit|]. (* l *)
+  rcondt {1} 25;[admit|]. (* l *)
 
   rcondt {2} 9;[intros &m;wp;rnd;wp;rnd;skip;trivial|]. (*good*)
   rcondf {2} 10;[admit|]. (* l condition *)
   rcondt {2} 10;[admit|]. (* l condition *)
   rcondt {2} 18;[admit|]. (* While *)
-  rcondt {2} 25;[admit|]. (* While *)
-  rcondf {2} 32;[admit|]. (* While *)
-  rcondt {2} 34;[admit|]. (* good *)
-  rcondf {2} 34;[admit|]. (* l *)
-  rcondt {2} 34;[admit|]. (* l *)
+  rcondt {2} 21;[admit|]. (* While *)
+  rcondf {2} 24;[admit|]. (* While *)
+  rcondt {2} 26;[admit|]. (* good *)
+  rcondf {2} 26;[admit|]. (* l *)
+  rcondt {2} 26;[admit|]. (* l *)
+
+  inline {1} Dkc.Dkc.encrypt.
+  inline {2} Dkc.Dkc.encrypt.
+
+  (*BEGIN CLEAN DKC*)
+  (*LOOP 1*)
+  (rcondt {1} 20;[admit|]). (* Dkc used *)
+  (rcondt {1} 21;[admit|]). (* Dkc not reusing *)
+  (rcondt {1} 22;[admit|]). (* Dkc not reusing *)
+  (rcondt {1} 23;[admit|]). (* Dkc not reusing *)
+  (rcondt {2} 21;[admit|]). (* Dkc used *)
+  (rcondt {2} 22;[admit|]). (* Dkc not reusing *)
+  (rcondt {2} 23;[admit|]). (* Dkc not reusing *)
+  (rcondt {2} 24;[admit|]). (* Dkc not reusing *)
+  (*LOOP 2*)
+  (rcondt {1} 33;[admit|]). (* Dkc used *)
+  (rcondt {1} 34;[admit|]). (* Dkc not reusing *)
+  (rcondt {1} 35;[admit|]). (* Dkc not reusing *) (*TODO: FALSE*)
+  (rcondt {1} 36;[admit|]). (* Dkc not reusing *)
+  (rcondt {2} 34;[admit|]). (* Dkc used *)
+  (rcondt {2} 35;[admit|]). (* Dkc not reusing *)
+  (rcondt {2} 36;[admit|]). (* Dkc not reusing *)
+  (rcondt {2} 37;[admit|]). (* Dkc not reusing *)
+  (*END CLEAN DKC*)
 
   wp.
-  call (answer{1}=answer{2}) (res{1} = res{2});[admit|].
+  call ((glob Adv){1} = (glob Adv){2}/\answer{1}=answer{2}) (res{1}=res{2}).
+    fun true;trivial.
   wp.
-  swap{1} [5..6] -3. (*rewrite tau*)
-  swap{1} 9 -5. (*rewrite tau*)
-  swap{1} 10 -5. (*t*)
-  swap{1} 38 -32. (*keyntau*)
+
+  (*init vals*)
+  swap [3..4] -2. (*maps*)
+  swap{1} [15..16] -12. (*i answers*)
+  swap{2} [16..17] -13. (*i answers*)
+  swap [9..10] -4. (*query*)
+  swap{1} 14 -13. (*good*)
+  swap{2} 15 -14. (*good*)
+  
+  (*tau{1}*)
+  swap{1} [10..12] -1. (*rewrite tau*)
+  swap{2} 13 -5. (*t*)
+
+  (*t{1}*)
+  swap{1} 13 -1. (*t*)
+  swap{2} [11..13] -1. (*rewrite tau*)
+
+  (*keyntau{1}*)
+  swap{1} 50 -37. (*keyntau*)
+  swap{2} [14..22] -1. (*keyt*)
+
+  (*keytau{1}*)
+  swap{2} [30..35] -2. (*keynt*)
+  
+
+  (*t{1}*)
+
 
   swap{2} 10 -9. (*t*)
+  swap{2} [6..7] -3. (*rewrite tau*)
+  swap{2} 10 -5. (*rewrite tau*)
 
-  swap{1} [6..7] -2. (*rewrite tau*)
-  swap{1} 10 -5. (*rewrite tau*)
+
+
+
+
+  swap{2} 38 -31. (*keyntau*)
+
   swap{2} 39 -30. (*key_nt_ntau*)
   swap{2} 39 -25. (*keyntau*)
   swap{1} 38 -25. (*keyntau*)
